Streamline guard verification in the examples.

books/kestrel/soft/workshop-paper-examples.lisp
@@ -43,16 +43,14 @@
 ; 1.2.1   Plain Functions
 
 (defun2 quad[?f] (?f) (x)
+  (declare (xargs :guard t))
   (?f (?f (?f (?f x)))))
 
-(verify-guards quad[?f]) ; omitted from the paper, for brevity
-
 (defun2 all[?p] (?p) (l)
+  (declare (xargs :guard t))
   (cond ((atom l) (null l))
         (t (and (?p (car l))
                 (all[?p] (cdr l))))))
-
-(verify-guards all[?p]) ; omitted from the paper, for brevity
 
 (defun2 map[?f_?p] (?f ?p) (l)
   (declare (xargs :guard (all[?p] l)))
@@ -61,11 +59,10 @@
                  (map[?f_?p] (cdr l))))))
 
 (defun2 fold[?f_?g] (?f ?g) (bt)
+  (declare (xargs :guard t))
   (cond ((atom bt) (?f bt))
         (t (?g (fold[?f_?g] (car bt))
                (fold[?f_?g] (cdr bt))))))
-
-(verify-guards fold[?f_?g]) ; omitted from the paper, for brevity
 
 ; 1.2.2  Choice Functions
 
@@ -79,22 +76,20 @@
           (implies (equal (?f x) (?f y))
                    (equal x y))))
 
-(verify-guards injective[?f]) ; omitted from the paper, for brevity
+(verify-guards injective[?f])
 
 ; 1.3  Instances of Second-Order Functions
 
 (defun wrap (x)
+  (declare (xargs :guard t))
   (list x))
-
-(verify-guards wrap) ; omitted from the paper, for brevity
 
 (defun-inst quad[wrap]
   (quad[?f] (?f . wrap)))
 
 (defun octetp (x)
+  (declare (xargs :guard t))
   (and (natp x) (< x 256)))
-
-(verify-guards octetp) ; omitted from the paper, for brevity
 
 (defun-inst all[octetp]
   (all[?p] (?p . octetp)))
@@ -106,15 +101,16 @@
   (fold[?f_?g] (?f . nfix) (?g . binary-+)))
 
 (defun twice (x)
+  (declare (xargs :guard t))
   (* 2 (fix x)))
-
-(verify-guards twice) ; omitted from the paper, for brevity
 
 (defun-inst fixpoint[twice]
   (fixpoint[?f] (?f . twice)))
 
 (defun-inst injective[quad[?f]] (?f)
   (injective[?f] (?f . quad[?f])))
+
+(verify-guards injective[quad[?f]])
 
 ; 1.4  Second-Order Theorems
 
@@ -155,7 +151,7 @@
                      (?io x (?f x))))
   :rewrite :direct)
 
-(verify-guards atom-io[?f_?io]) ; omitted from the paper, for brevity
+(verify-guards atom-io[?f_?io])
 
 (defun-sk2 consp-io[?g_?io] (?g ?io) ()
   (forall (x y1 y2)
@@ -165,7 +161,7 @@
                    (?io x (?g y1 y2))))
   :rewrite :direct)
 
-(verify-guards consp-io[?g_?io]) ; omitted from the paper, for brevity
+(verify-guards consp-io[?g_?io])
 
 (defthm fold-io[?f_?g_?io]
   (implies (and (atom-io[?f_?io])
@@ -180,16 +176,19 @@
 (defun-inst injective[quad[wrap]]
   (injective[quad[?f]] (?f . wrap)))
 
+(verify-guards injective[quad[wrap]])
+
 (defun-inst injective[wrap]
   (injective[?f] (?f . wrap)))
+
+(verify-guards injective[wrap])
 
 (defthm-inst injective[quad[wrap]]-when-injective[wrap]
   (injective[quad[?f]]-when-injective[?f] (?f . wrap)))
 
 ; 2  Use in Program Refinement
 
-; to keep the program refinement example shorter:
-(set-verify-guards-eagerness 0) ; omitted from the paper, for brevity
+(set-verify-guards-eagerness 0) ; to keep the program refinement example shorter
 
 ; 2.1  Specifications as Second-Order Predicates
 
